WIP, something working with step functions etc, figuring out induction

cava/Cava/Core/CavaClass.v
@@ -16,12 +16,400 @@
 
 Require Import Cava.Core.Netlist.
 Require Import Cava.Core.Signal.
-Require Import Cava.Util.Tuple.
-
-Local Open Scope type_scope.
 
 (**** IMPORTANT: if you make changes to the API of these definitions, or add new
       ones, make sure you update the reference at docs/reference.md! ****)
+
+(* combines two types while not duplicating Void values *)
+Definition tpair_min (t1 t2 : type) : type :=
+  match t1, t2 with
+  | tone Void, t2 => t2
+  | t1, tone Void => t1
+  | t1, t2 => tpair t1 t2
+  end.
+Infix "**" := tpair_min (at level 40) : signal_scope.
+Definition tprod_min {t1 t2 : type} : value t1 -> value t2 -> value (tpair_min t1 t2) :=
+  match t1, t2 with
+  | tone Void, _ => fun _ y => y
+  | _, tone Void => fun x _ => x
+  | _,_ => fun x y => (x,y)
+  end.
+Definition tsplit {t1 t2 : type} : value (t1 ** t2) -> value t1 * value t2 :=
+  match t1, t2 with
+  | tone Void, _ => fun x => (tt, x)
+  | _, tone Void => fun x => (x, tt)
+  | _,_ => fun x => x
+  end.
+
+(* A PHOAS-style expression representing a circuit *)
+Inductive CircuitExpr {var : type -> Type} : type -> type -> Type :=
+(* Name and reference wires *)
+| Var : forall {t}, var t -> CircuitExpr Void t
+| Bind : forall {t u s1 s2}, CircuitExpr s1 t -> (var t -> CircuitExpr s2 u) -> CircuitExpr (s1 ** s2) u
+(* Constants *)
+| Constant : bool -> CircuitExpr Void Bit
+| ConstantV : forall {A n}, Vector.t (signal A) n -> CircuitExpr Void (Vec A n)
+| DefaultSignal : forall t, CircuitExpr Void t
+(* Tuples *)
+| Prod : forall {t u s1 s2}, CircuitExpr s1 t -> CircuitExpr s2 u -> CircuitExpr (s1 ** s2) (t * u)
+| Fst : forall {t u s}, CircuitExpr s (t ** u) -> CircuitExpr s t
+| Snd : forall {t u s}, CircuitExpr s (t ** u) -> CircuitExpr s u
+(* Registers *)
+| Delay : forall {t s}, value t -> CircuitExpr s t -> CircuitExpr (t ** s) t
+| LoopDelay : forall {o s t}, value t -> (var t -> CircuitExpr s (t ** o)) -> CircuitExpr (t ** s) o
+.
+Global Arguments CircuitExpr : clear implicits.
+
+(*
+  (* Default values. *)
+  defaultSignal : forall {t: SignalType}, signal t;
+  (* SystemVerilog primitive gates *)
+  inv : signal Bit -> cava (signal Bit);
+  and2 : signal Bit * signal Bit -> cava (signal Bit);
+  nand2 : signal Bit * signal Bit -> cava (signal Bit);
+  or2 : signal Bit * signal Bit -> cava (signal Bit);
+  nor2 : signal Bit * signal Bit -> cava (signal Bit);
+  xor2 : signal Bit * signal Bit -> cava (signal Bit);
+  xnor2 : signal Bit * signal Bit -> cava (signal Bit);
+  buf_gate : signal Bit -> cava (signal Bit); (* Corresponds to the SystemVerilog primitive gate 'buf' *)
+  (* Xilinx UNISIM FPGA gates *)
+  lut1 : (bool -> bool) -> signal Bit -> cava (signal Bit); (* 1-input LUT *)
+  lut2 : (bool -> bool -> bool) -> (signal Bit * signal Bit) -> cava (signal Bit); (* 2-input LUT *)
+  lut3 : (bool -> bool -> bool -> bool) -> signal Bit * signal Bit * signal Bit -> cava (signal Bit); (* 3-input LUT *)
+  lut4 : (bool -> bool -> bool -> bool -> bool) -> (signal Bit * signal Bit * signal Bit * signal Bit) ->
+         cava (signal Bit); (* 4-input LUT *)
+  lut5 : (bool -> bool -> bool -> bool -> bool -> bool) ->
+         (signal Bit * signal Bit * signal Bit * signal Bit * signal Bit) -> cava (signal Bit); (* 5-input LUT *)
+  lut6 : (bool -> bool -> bool -> bool -> bool -> bool -> bool) ->
+         signal Bit * signal Bit * signal Bit * signal Bit * signal Bit * signal Bit -> cava (signal Bit); (* 6-input LUT *)
+  xorcy : signal Bit * signal Bit -> cava (signal Bit); (* Xilinx fast-carry UNISIM with arguments O, CI, LI *)
+  muxcy : signal Bit -> signal  Bit -> signal Bit -> cava (signal Bit); (* Xilinx fast-carry UNISIM with arguments O, CI, DI, S *)
+  (* Converting to/from Vector.t *)
+  unpackV : forall {t : SignalType} {s : nat}, signal (Vec t s) -> cava (Vector.t (signal t) s);
+  packV : forall {t : SignalType} {s : nat} , Vector.t (signal t) s -> cava (signal (Vec t s));
+  (* Dynamic indexing *)
+  indexAt : forall {t : SignalType} {sz isz: nat},
+            signal (Vec t sz) ->     (* A vector of n elements of type signal t *)
+            signal (Vec Bit isz) ->  (* A bit-vector index of size isz bits *)
+            cava (signal t);                (* The indexed value of type signal t *)
+  (* Synthesizable arithmetic operations. *)
+  unsignedAdd : forall {a b : nat}, signal (Vec Bit a) * signal (Vec Bit b) ->
+                cava (signal (Vec Bit (1 + max a b)));
+  unsignedMult : forall {a b : nat}, signal (Vec Bit a) * signal (Vec Bit b)->
+                cava (signal (Vec Bit (a + b)));
+  (* Synthesizable relational operators *)
+  greaterThanOrEqual : forall {a b : nat}, signal (Vec Bit a) * signal (Vec Bit b) ->
+                      cava (signal Bit);
+  (* Naming for sharing. *)
+  localSignal : forall {t : SignalType}, signal t -> cava (signal t);
+  (* Hierarchy *)
+  instantiate : forall (intf: CircuitInterface),
+                let inputs := map (port_signal signal) (circuitInputs intf) in
+                let outputs := map (port_signal signal) (circuitOutputs intf) in
+                curried inputs (cava (tupled' outputs)) ->
+                 tupled' inputs -> cava (tupled' outputs);
+  (* Instantiation of black-box components which return default values. *)
+  blackBox : forall (intf: CircuitInterface),
+             tupled' (map (port_signal signal) (circuitInputs intf)) ->
+             cava (tupled' (map (port_signal signal) (circuitOutputs intf)));
+}.
+*)
+Definition Circuit i o s : Type := forall var, var i -> CircuitExpr var s o.
+
+Fixpoint step {t s} (c : CircuitExpr value s t)
+  : value s -> value s * value t :=
+  match c in CircuitExpr _ s t return value s -> value s * value t with
+  | Var x => fun s => (s, x)
+  | Bind x f =>
+    fun s =>
+      let '(xs, fs) := tsplit s in
+      let '(xs, xo) := step x xs in
+      let '(fs, fo) := step (f xo) fs in
+      (tprod_min xs fs, fo)
+  | Constant x => fun _ => (tt, x)
+  | ConstantV x => fun _ => (tt, x)
+  | DefaultSignal t => fun _ => (tt, default_value t)
+  | Prod x y =>
+    fun s =>
+      let '(xs, ys) := tsplit s in
+      let '(xs, xo) := step x xs in
+      let '(ys, yo) := step y ys in
+      (tprod_min xs ys, (xo, yo))
+  | Fst x =>
+    fun s =>
+      let '(s, xo) := step x s in
+      (s, fst (tsplit xo))
+  | Snd x =>
+    fun s =>
+      let '(s, xo) := step x s in
+      (s, snd (tsplit xo))
+  | Delay _ x =>
+    fun s =>
+      let '(s, xs) := tsplit s in
+      let '(xs, xo) := step x xs in
+      (tprod_min xo xs, s)
+  | LoopDelay _ x =>
+    fun s =>
+      let '(r, xs) := tsplit s in
+      let '(xs, xo) := step (x r) xs in
+      let '(r, o) := tsplit xo in
+      (tprod_min r xs, o)
+  end.
+
+Fixpoint reset_state {t s} (c : CircuitExpr value s t) : value s :=
+  match c in CircuitExpr _ s t return value s with
+  | Var x => tt
+  | Bind x f => tprod_min (reset_state x) (reset_state (f (default_value _)))
+  | Constant x => tt
+  | ConstantV x => tt
+  | DefaultSignal t => tt
+  | Prod x y => tprod_min (reset_state x) (reset_state y)
+  | Fst x => reset_state x
+  | Snd x => reset_state x
+  | Delay r x => tprod_min r (reset_state x)
+  | LoopDelay r x => tprod_min r (reset_state (x (default_value _)))
+  end.
+
+
+Print CircuitExpr.
+(* Says that two circuit expressions are constructed in exactly the same way *)
+Inductive expr_equiv : forall {s t}, CircuitExpr value s t -> CircuitExpr value s t -> Prop :=
+| equiv_Var : forall t (x : value t), expr_equiv (Var x) (Var x)
+| equiv_Bind :
+    forall t u s1 s2 (x : CircuitExpr value s1 t) (f g : value t -> CircuitExpr value s2 u),
+      (forall y, expr_equiv (f y) (g y)) ->
+      expr_equiv (Bind x f) (Bind x g)
+| equiv_Constant : forall b, expr_equiv (Constant b) (Constant b)
+| equiv_ConstantV : forall A n (v : Vector.t (signal A) n), expr_equiv (ConstantV v) (ConstantV v)
+| equiv_DefaultSignal : forall t, expr_equiv (DefaultSignal t) (DefaultSignal t)
+| equiv_Prod :
+    forall t u s1 s2 (x1 x2 : CircuitExpr value s1 t) (y1 y2 : CircuitExpr value s2 u),
+      expr_equiv x1 x2 ->
+      expr_equiv y1 y2 ->
+      expr_equiv (Prod x1 y1) (Prod x2 y2)
+| equiv_Fst :
+    forall t u s (x1 x2 : CircuitExpr value s (t ** u)),
+      expr_equiv x1 x2 ->
+      expr_equiv (Fst x1) (Fst x2)
+| equiv_Snd :
+    forall t u s (x1 x2 : CircuitExpr value s (t ** u)),
+      expr_equiv x1 x2 ->
+      expr_equiv (Snd x1) (Snd x2)
+| equiv_Delay :
+    forall t s r (x1 x2 : CircuitExpr value s t),
+      expr_equiv x1 x2 ->
+      expr_equiv (Delay r x1) (Delay r x2)
+| equiv_LoopDelay :
+    forall o s t r (x1 x2 : value t -> CircuitExpr value s (t ** o)),
+      (forall y, expr_equiv (x1 y) (x2 y)) ->
+      expr_equiv (LoopDelay r x1) (LoopDelay r x2)
+.
+
+Lemma reset_state_ext {i o s} (c : value i -> CircuitExpr value s o) x y :
+  (
+  reset_state (c x) = reset_state (c y).
+Proof.
+  induction (c x).
+  all:cbn.
+Qed.
+
+Definition test : Circuit (Vec Bit 4) (Vec Bit 4 * Vec Bit 4) Void :=
+  fun var x => Prod (Var x) (Var x).
+Definition test2 : Circuit (Vec Bit 4) (Vec Bit 4 * Vec Bit 4) (Vec Bit 4) :=
+  fun var x => Bind (Delay (t:=Vec Bit 4) (Vector.const false 4) (Var x))
+                 (fun y => Prod (Var x) (Var y)).
+
+Require Import Cava.Util.List.
+Definition simulate {i o s} (c : Circuit i o s) (input : list (value i)) : list (value o) :=
+  fold_left_accumulate (fun s x => step (c value x) s) input (reset_state (c value (default_value i))).
+Import Vector.VectorNotations.
+Compute simulate test2 (map (B:=value (Vec Bit 4)) (fun i => Ndigits.N2Bv_sized 4 (BinNat.N.of_nat i)) (seq 0 3)).
+
+
+
+
+
+
+
+
+
+
+
+
+
+
+
+
+
+
+(* A PHOAS-style expression representing a circuit *)
+Inductive CircuitExpr {var : type -> Type} : type -> type -> Type :=
+| Var : forall {t}, var t -> CircuitExpr Void t
+| Abs : forall {t u v}, (var t -> CircuitExpr u v) -> CircuitExpr (t * u) v
+| App : forall {t u}, CircuitExpr t u -> CircuitExpr Void t -> CircuitExpr Void u
+                                                                    (*
+| Bind :
+    forall {t u v},
+      CircuitExpr Void t -> (var t -> CircuitExpr u v) ->
+      CircuitExpr u v
+*)
+| ConstantBit : bool -> CircuitExpr Void Bit
+| And : CircuitExpr Void (Bit * Bit) -> CircuitExpr Void Bit
+| Fst : forall {t u}, CircuitExpr Void (t * u) -> CircuitExpr Void t
+| Snd : forall {t u}, CircuitExpr Void (t * u) -> CircuitExpr Void u
+| Prod : forall {t u}, CircuitExpr Void t -> CircuitExpr Void u ->
+                  CircuitExpr Void (t * u)
+.
+Global Arguments CircuitExpr : clear implicits.
+
+Definition Bind {var t u v} (x : CircuitExpr var Void t) (f : var t -> CircuitExpr var u v)
+  : CircuitExpr var u v :=
+  Abs
+    (fun y => App (Abs f) (Prod x (Var y))).
+Check (Abs
+         (fun i1 : value (Vec Bit 4) =>
+            Abs
+              (fun i2 : value (Vec Bit 2) =>
+                 Prod (Prod (Var i1) (Constant true)) (Var i2)))).
+Check (Abs
+         (fun i1 : value (Vec Bit 4) =>
+            Abs
+              (fun i2 : value (Vec Bit 2) =>
+                 Bind (Prod (Var i1) (Constant true))
+                      (fun x => And (Prod (Snd (Var x)) (Snd (Var x))))))).
+
+Fixpoint cstate {i o} (c : CircuitExpr value i o) : type :=
+  match c with
+  | Var _ => Void
+  | Bind x f => tcombine (cstate x) (cstate f)
+  | BindInput f => cstate f
+  | Constant x => Void
+  | And => Void
+  | Fst => Void
+  | Snd => Void
+  | Prod x y => 
+
+(*
+Inductive interface : Type :=
+| ione (o : type)
+| iarrow (i o : type)
+.
+
+(* A PHOAS-style expression representing a circuit *)
+Inductive CircuitExpr {var : type -> Type} : interface -> Type :=
+| Var : forall {t}, var t -> CircuitExpr (ione t)
+| Abs : forall {t u}, (var t -> CircuitExpr (ione u)) -> CircuitExpr (iarrow t u)
+| App : forall {t u}, CircuitExpr (iarrow t u) -> CircuitExpr (ione t) -> CircuitExpr (ione u)
+| Input : forall t, CircuitExpr (ione t)
+| Bind :
+    forall {t u}, CircuitExpr (ione t) -> (var t -> CircuitExpr (ione u)) -> CircuitExpr (ione u)
+| Constant : bool -> CircuitExpr (ione Bit)
+| Prod : forall {t u}, CircuitExpr (ione t) -> CircuitExpr (ione u) -> CircuitExpr (ione (t * u))
+| Fst : forall {t u}, CircuitExpr (ione (t * u)) -> CircuitExpr (ione t)
+| Snd : forall {t u}, CircuitExpr (ione (t * u)) -> CircuitExpr (ione u)
+| Delay : forall {t}, CircuitExpr (ione t) -> CircuitExpr (ione t)
+.
+Global Arguments CircuitExpr : clear implicits.
+
+Definition Circuit t : Type := forall var, CircuitExpr var t.
+
+Check (fun var => Prod (var:=var) (Input (Vec Bit 4)) (Constant true)).
+Check (fun var => Bind (var:=var)
+                    (Input (Vec Bit 4))
+                    (fun x => Prod (Var x) (Var x))).
+*)
+
+
+(* A PHOAS-style expression representing a circuit *)
+Inductive CircuitExpr {var : type -> Type} : type -> Type :=
+| Var : forall {t}, var t -> CircuitExpr t
+| Bind : forall {t u}, CircuitExpr t -> (var t -> CircuitExpr u) -> CircuitExpr u
+| Input : forall t, CircuitExpr t
+| Constant : bool -> CircuitExpr Bit
+| Prod : forall {t u}, CircuitExpr t -> CircuitExpr u -> CircuitExpr (t * u)
+| Fst : forall {t u}, CircuitExpr (t * u) -> CircuitExpr t
+| Snd : forall {t u}, CircuitExpr (t * u) -> CircuitExpr u
+| Delay : forall {t}, CircuitExpr t -> CircuitExpr t
+.
+Global Arguments CircuitExpr : clear implicits.
+
+Definition Circuit t : Type := forall var, CircuitExpr var t.
+
+Check (fun var => Prod (var:=var) (Input (Vec Bit 4)) (Constant true)).
+Check (fun var => Bind (var:=var)
+                    (Input (Vec Bit 4))
+                    (fun x => Prod (Var x) (Var x))).
+
+Fixpoint circuit_input {t} (c : CircuitExpr (fun _ => unit) t) : type :=
+  match c with
+  | Var x => Void
+  | Input t => t
+  | Bind x f => tcombine (circuit_input x) (circuit_input (f tt))
+  | Constant x => Void
+  | Prod x y => tcombine (circuit_input x) (circuit_input y)
+  | Fst x => circuit_input x
+  | Snd x => circuit_input x
+  | Delay x => circuit_input x
+  end.
+
+Definition test : Circuit _ :=
+  fun var => Bind (Input (Vec Bit 4))
+               (fun x => Prod (Var x) (Var x)).
+Compute circuit_input (test _).
+Definition test2 : Circuit _ :=
+  fun var => Bind (Input (Vec Bit 4))
+               (fun x => Bind (Delay (Var x))
+                           (fun y => Prod (Var x) (Var y))).
+Compute circuit_input (test2 _).
+
+Fixpoint circuit_state {t} (c : CircuitExpr (fun _ => unit) t) : type :=
+  match c with
+  | Var x => Void
+  | Input t => Void
+  | Bind x f => tcombine (circuit_state x) (circuit_state (f tt))
+  | Constant x => Void
+  | Prod x y => tcombine (circuit_state x) (circuit_state y)
+  | Fst x => circuit_state x
+  | Snd x => circuit_state x
+  | @Delay _ t x => t
+  end.
+
+Compute circuit_state (test _).
+Compute circuit_state (test2 _).
+
+Definition step {t} (c : Circuit t)
+           (state : value (circuit_state (c _)))
+           (input : value (circuit_input (c _)))
+  : value t * value (circuit_state (c _)).
+  match (c value) with
+  | 
+
+
+(* A PHOAS-style expression representing a circuit *)
+Inductive CircuitExpr {var : type -> Type} : type -> type -> Type :=
+| Var : forall {t}, var t -> CircuitExpr Void t
+| Bind :
+    forall {t u v}, CircuitExpr Void t -> (var t -> CircuitExpr u v) ->
+               CircuitExpr u v
+| BindInput :
+    forall {t u v}, (var t -> CircuitExpr u v) -> CircuitExpr (u * t) v
+| Constant : bool -> CircuitExpr Void Bit
+| And : CircuitExpr (Bit * Bit) Bit
+| Fst : forall {t u}, CircuitExpr (t * u) t
+| Snd : forall {t u}, CircuitExpr (t * u) u
+| Prod : forall {t u}, CircuitExpr Void t -> CircuitExpr Void u ->
+                  CircuitExpr Void (t * u)
+.
+Global Arguments CircuitExpr : clear implicits.
+
+Check (BindInput
+         (fun i1 : value (Vec Bit 4) =>
+            BindInput
+              (fun i2 : value (Vec Bit 2) =>
+                 Prod (Prod (Var i1) (Constant true)) (Var i2)))).
+
+Fixpoint cstate {i o} (c : CircuitExpr value i o)
+
 
 Definition port_signal signal port : Type := signal (port_type port).
 
